proofs and hints

code/experimental/salsa-family/Hacl.Impl.Chacha20.Vec128.fst
@@ -702,37 +702,6 @@ let chacha20_core3 log k0 k1 k2 st =
   let h3 = ST.get() in
   ()
 
-(* [@ "c_inline"] *)
-(* val chacha20_block: *)
-(*   log:log_t -> *)
-(*   stream_block:uint8_p{length stream_block = 64} -> *)
-(*   st:state{disjoint st stream_block} -> *)
-(*   ctr:UInt32.t -> *)
-(*   Stack log_t *)
-(*     (requires (fun h -> live h stream_block /\ invariant log h st)) *)
-(*     (ensures  (fun h0 updated_log h1 -> live h1 stream_block /\ modifies_1 stream_block h0 h1 /\ *)
-(*       invariant updated_log h1 st /\ modifies_2 stream_block st h0 h1 *)
-(*       /\ (let block = reveal_sbytes (as_seq h1 stream_block) in *)
-(*          match Ghost.reveal log, Ghost.reveal updated_log with *)
-(*          | MkLog k n, MkLog k' n' -> *)
-(*              block == Spec.chacha20_block k n (U32.v ctr) /\ k == k' /\ n == n'))) *)
-(* [@ "c_inline"] *)
-(* let chacha20_block log stream_block st = *)
-(*   push_frame(); *)
-(*   let h0 = ST.get() in *)
-(*   let k = Buffer.create zero 4ul in *)
-(*   let h1 = ST.get() in *)
-(*   no_upd_lemma_0 h0 h1 stream_block; *)
-(*   no_upd_lemma_0 h0 h1 st; *)
-(*   chacha20_core k st; *)
-(*   let h2 = ST.get() in *)
-(*   no_upd_lemma_1 h1 h2 k stream_block; *)
-(*   no_upd_lemma_1 h1 h2 k st; *)
-(*   state_to_key_block stream_block k; *)
-(*   let h3 = ST.get() in *)
-(*   pop_frame(); *)
-(*   Ghost.elift1 (fun l -> match l with | MkLog k n -> MkLog k n) log'   *)
-
 
 [@ "c_inline"]
 val chacha20_block:
@@ -822,21 +791,6 @@ let update_last log output plain len st =
   let h5 = ST.get() in
   ()
 
-
-(* val load_bytes_to_state: *)
-(*   st:state -> *)
-(*   plain:uint8_p{length plain = 64 /\ disjoint st plain} -> *)
-(*   Stack unit *)
-(*     (requires (fun h -> live h st /\ live h plain)) *)
-(*     (ensures (fun h0 _ h1 -> live h0 st /\ live h0 plain /\ *)
-(*       live h1 st /\ modifies_1 st h0 h1 /\ ( *)
-(*       let st = as_seq h1 st in *)
-(*       let plain = as_seq h0 plain in *)
-(*       vec_as_seq (Seq.index st 0) == Spec.Lib.uint32s_from_le 4 (Seq.slice plain 0 16) /\ *)
-(*       vec_as_seq (Seq.index st 1) == Spec.Lib.uint32s_from_le 4 (Seq.slice plain 16 32) /\ *)
-(*       vec_as_seq (Seq.index st 2) == Spec.Lib.uint32s_from_le 4 (Seq.slice plain 32 48) /\ *)
-(*       vec_as_seq (Seq.index st 3) == Spec.Lib.uint32s_from_le 4 (Seq.slice plain 48 64) ))) *)
-(* let load_bytes_to_state st plain = *)  
 
 #reset-options "--max_fuel 0 --z3rlimit 20"
 
@@ -1041,10 +995,6 @@ val xor_block:
       let stbytes = FStar.Seq.(Spec.Lib.uint32s_to_le 16 (
                                vec_as_seq (Seq.index st 0) @| vec_as_seq (Seq.index st 1) @|
                                vec_as_seq (Seq.index st 2) @| vec_as_seq (Seq.index st 3))) in
-      (* let stbytes = FStar.Seq.(Spec.Lib.uint32s_to_le 4 (vec_as_seq (Seq.index st 0)) @| *)
-      (*                          Spec.Lib.uint32s_to_le 4 (vec_as_seq (Seq.index st 1)) @| *)
-      (*                          Spec.Lib.uint32s_to_le 4 (vec_as_seq (Seq.index st 2)) @| *)
-      (*                          Spec.Lib.uint32s_to_le 4 (vec_as_seq (Seq.index st 3))) in *)
       output == Spec.Loops.seq_map2 UInt8.logxor plain stbytes) ))
 let xor_block output plain st =
   let h0 = ST.get() in
@@ -1303,12 +1253,11 @@ val update3':
         invariant log' h1 st /\
         Seq.slice (as_seq h1 output) 0 (192 * U32.v i + 192) == Spec.CTR3.counter_mode_blocks3 k n (U32.v ctr) plain (U32.v i + 1)))))
 
-#reset-options "--max_fuel 0 --z3rlimit 200"
+#reset-options "--max_fuel 0 --z3rlimit 300"
 
 let update3' log output plain len st i =
   let h0  = ST.get() in
   let h   = ST.get() in
-  (* Seq.lemma_eq_intro (Seq.slice (as_seq h0 plain) 0 (192 * U32.v i + 192)) *)
   let out_sub      = Buffer.sub output 0ul U32.(192ul *^ i +^ 192ul) in
   let plain_sub    = Buffer.sub plain 0ul U32.(192ul *^ i +^ 192ul)  in
   let out_block    = Buffer.sub output U32.(192ul *^ i) 192ul        in
@@ -1322,12 +1271,23 @@ let update3' log output plain len st i =
   Seq.lemma_eq_intro (as_seq h plain_block) (Seq.slice (as_seq h0 plain) (192 * U32.v i) (192 * U32.v i + 192));
   Seq.lemma_eq_intro FStar.Seq.(slice (as_seq h0 plain) 0 (192 * U32.v i) @| slice (as_seq h0 plain) (192 * U32.v i) (192 * U32.v i + 192))
                      (Seq.slice (as_seq h0 plain) 0 (192 * U32.v i + 192));
+  Seq.lemma_eq_intro (Seq.slice (as_seq h plain_sub) (192 * U32.v i) (192 * U32.v i + 192))
+                     (as_seq h plain_block);
+  Seq.lemma_eq_intro (Seq.slice (as_seq h plain_sub) (0) (192 * U32.v i))
+                     (as_seq h plain_prefix);
   let log' = log_incrn log U32.(3ul *^ i) in
   Spec.CTR3.lemma_counter_mode_blocks3_def1 (Ghost.reveal log).k (Ghost.reveal log).n (U32.v (Ghost.reveal log).ctr ) (Seq.slice (as_seq h0 plain) 0 (192 * U32.v i + 192)) (U32.v i + 1);
   update3 log' out_block plain_block st;
   let h'  = ST.get() in
+  Seq.lemma_eq_intro (Seq.slice (as_seq h' out_sub) (192 * U32.v i) (192 * U32.v i + 192))
+                     (as_seq h' out_block);
+  Seq.lemma_eq_intro (Seq.slice (as_seq h' out_sub) (0) (192 * U32.v i))
+                     (as_seq h' out_prefix);
   Seq.lemma_eq_intro FStar.Seq.(slice (as_seq h' output) 0 (192 * U32.v i) @| slice (as_seq h' output) (192 * U32.v i) (192 * U32.v i + 192))
                        (Seq.slice (as_seq h' output) 0 (192 * U32.v i + 192));
+  Seq.lemma_eq_intro (Seq.append (as_seq h out_prefix) (as_seq h' out_block))
+                     (match Ghost.reveal log with | MkLog k n c ->
+                       Spec.CTR3.counter_mode_blocks3 k n (U32.v c) (as_seq h plain_sub) (U32.v i+1));
   no_upd_lemma_2 h h' out_block st out_prefix;
   no_upd_lemma_2 h h' out_block st plain_prefix;
   no_upd_lemma_2 h h' out_block st plain_block;
@@ -1338,12 +1298,17 @@ let update3' log output plain len st i =
   no_upd_lemma_1 h' h'' st output;
   no_upd_lemma_1 h' h'' st plain;
   no_upd_lemma_1 h' h'' st out_block;
+  no_upd_lemma_1 h' h'' st out_prefix;
+  no_upd_lemma_1 h' h'' st out_sub;
+  no_upd_lemma_1 h' h'' st plain_block;
+  no_upd_lemma_1 h' h'' st plain_prefix;
+  no_upd_lemma_1 h' h'' st plain_sub;
   assert(match Ghost.reveal log with | MkLog k n c ->
     let c' = U32.(c +^ 3ul *^ (i+^1ul)) in
     let log' = Ghost.hide (MkLog k n c') in
     invariant log' h'' st);
   Seq.lemma_eq_intro (as_seq h'' out_sub) (Seq.append (as_seq h out_prefix) (as_seq h' out_block));
-  Seq.lemma_eq_intro (as_seq h'' out_sub)
+  Seq.lemma_eq_intro (Seq.slice (as_seq h'' output) 0 (192 * U32.v i + 192))
                      (match Ghost.reveal log with | MkLog k n c ->
                       Spec.CTR3.counter_mode_blocks3 k n (UInt32.v c) (Seq.slice (as_seq h0 plain) 0 (192 * U32.v i + 192)) (U32.v i+1))
 
@@ -1369,13 +1334,21 @@ val chacha20_counter_mode_blocks3:
 
 #reset-options "--max_fuel 0 --z3rlimit 200"
 
+val lemma_modifies_nothing_modifies_2:
+  h:HyperStack.mem ->
+  out:uint8_p{live h out} ->
+  st:state{live h st /\ disjoint st out} ->
+  Lemma (modifies_2 out st h h)
+let lemma_modifies_nothing_modifies_2 h out st =
+  lemma_intro_modifies_2 out st h h
+
+#reset-options "--max_fuel 0 --z3rlimit 300"
+
 let chacha20_counter_mode_blocks3 log output plain len st =
-  let len3 = U32.(len /^ 3ul) in
-  let rest3 = U32.(len %^ 3ul) in
   let h0 = ST.get() in
-  let inv (h1:HyperStack.mem) (i:nat{i <= UInt32.v len3}) : Type0 =
+  let inv (h1:HyperStack.mem) (i:nat) : Type0 =
     live h1 output /\ live h1 plain /\ live h1 st /\ modifies_2 output st h0 h1 /\
-    as_seq h1 plain == as_seq h0 plain /\
+    as_seq h1 plain == as_seq h0 plain /\ i <= U32.v len /\
     (match Ghost.reveal log with | MkLog k n c ->
      let c' = U32.(c +^ 3ul *^ UInt32.uint_to_t i) in
      let log' = Ghost.hide (MkLog k n c') in
@@ -1383,50 +1356,23 @@ let chacha20_counter_mode_blocks3 log output plain len st =
      invariant log' h1 st /\
      Seq.slice (as_seq h1 output) 0 (192 * i) == Spec.CTR3.counter_mode_blocks3 k n (UInt32.v c) plain i)
   in
-  let f' (i:UInt32.t{0 <= U32.v i /\ U32.v i < U32.v len3}) : Stack unit
+  let f' (i:UInt32.t{0 <= U32.v i /\ U32.v i < U32.v len}) : Stack unit
     (requires (fun h -> inv h (U32.v i)))
     (ensures (fun h0 _ h1 -> inv h1 (U32.v i + 1)))
   =
     let h   = ST.get() in
-    (* Seq.lemma_eq_intro (Seq.slice (as_seq h0 plain) 0 (192 * U32.v i + 192)) *)
-    let out_sub      = Buffer.sub output 0ul U32.(192ul *^ i +^ 192ul) in
-    let plain_sub    = Buffer.sub plain 0ul U32.(192ul *^ i +^ 192ul)  in
-    let out_block    = Buffer.sub output U32.(192ul *^ i) 192ul        in
-    let plain_block  = Buffer.sub plain U32.(192ul *^ i) 192ul         in
-    let out_prefix   = Buffer.sub output 0ul U32.(192ul *^ i)          in
-    let plain_prefix = Buffer.sub plain 0ul U32.(192ul *^ i)           in
-    let plain'       = Buffer.sub plain 0ul U32.(192ul *^ i +^ 192ul)  in
-    let output'      = Buffer.sub output 0ul U32.(192ul *^ i +^ 192ul) in
-    Seq.lemma_eq_intro (as_seq h plain_prefix) (Seq.slice (as_seq h0 plain) 0 (192 * U32.v i));
-    Seq.lemma_eq_intro (as_seq h plain_block) (Seq.slice (as_seq h0 plain) (192 * U32.v i) (192 * U32.v i + 192));
-    Seq.lemma_eq_intro FStar.Seq.(slice (as_seq h0 plain) 0 (192 * U32.v i) @| slice (as_seq h0 plain) (192 * U32.v i) (192 * U32.v i + 192))
-                       (Seq.slice (as_seq h0 plain) 0 (192 * U32.v i + 192));
-    let log' = log_incrn log U32.(3ul *^ i) in
-    Spec.CTR3.lemma_counter_mode_blocks3_def1 (Ghost.reveal log').k (Ghost.reveal log').n (U32.v (Ghost.reveal log').ctr ) (Seq.slice (as_seq h0 plain) 0 (192 * U32.v i + 192)) (U32.v i + 1);
-    update3 log' out_block plain_block st;
+    update3' log output plain len st i;
     let h'  = ST.get() in
-    Seq.lemma_eq_intro FStar.Seq.(slice (as_seq h' output) 0 (192 * U32.v i) @| slice (as_seq h' output) (192 * U32.v i) (192 * U32.v i + 192))
-                       (Seq.slice (as_seq h' output) 0 (192 * U32.v i + 192));
-    no_upd_lemma_2 h h' out_block st out_prefix;
-    no_upd_lemma_2 h h' out_block st plain_prefix;
-    no_upd_lemma_2 h h' out_block st plain_block;
-    no_upd_lemma_2 h h' out_block st plain;
-    let log'' = log_incrn log' 2ul in
-    state_incr log'' st;
-    let h'' = ST.get() in
-    no_upd_lemma_1 h' h'' st output;
-    no_upd_lemma_1 h' h'' st plain;
-    no_upd_lemma_1 h' h'' st out_block;
-    assert(match Ghost.reveal log with | MkLog k n c ->
-      let c' = U32.(c +^ 3ul *^ (i+^1ul)) in
-      let log' = Ghost.hide (MkLog k n c') in
-      invariant log' h'' st);
-    Seq.lemma_eq_intro (Seq.slice (as_seq h'' output) 0 (192 * U32.v i + 192))
-                       (match Ghost.reveal log with | MkLog k n c ->
-                        Spec.CTR3.counter_mode_blocks3 k n (UInt32.v c) (Seq.slice (as_seq h0 plain) 0 (192 * U32.v i + 192)) (U32.v i+1))
+    ()
     in
-  admit();
-  C.Loops.for 0ul len3 inv f'
+  Seq.lemma_eq_intro (Seq.slice (as_seq h0 output) 0 0) (Seq.createEmpty);
+  Spec.CTR3.lemma_counter_mode_blocks3_def0 (Ghost.reveal log).k (Ghost.reveal log).n (U32.v (Ghost.reveal log).ctr) (Seq.slice (as_seq h0 plain) 0 0);
+  C.Loops.for 0ul len inv f';
+  let h1 = ST.get() in
+  Seq.lemma_eq_intro (as_seq h1 output) (Seq.slice (as_seq h1 output) 0 (length output));
+  Seq.lemma_eq_intro (as_seq h0 plain) (Seq.slice (as_seq h0 plain) 0 (length plain));
+  Seq.lemma_eq_intro (as_seq h1 output)
+                     (Spec.CTR3.counter_mode_blocks3 (Ghost.reveal log).k (Ghost.reveal log).n (U32.v (Ghost.reveal log).ctr) (as_seq h0 plain) (U32.v len))
 
 
 #reset-options "--max_fuel 0 --z3rlimit 20"
